I proved left_expand_mat_star_blocks.

matrix.v
@@ -48,7 +48,7 @@ Definition mat_dot {m n p} (a : mat m n) (b : mat n p) i j : X :=
 Definition mat_mul {m n p} (a : mat m n) (b : mat n p) : mat m p :=
   mat_build (mat_dot a b).
 
-Definition mat_one {n} :=
+Definition mat_id {n} :=
   mat_build (λ i j : fin n, if i =? j then 1 else 0).
 
 Notation "a × b" := (mat_mul a b) (at level 40).
@@ -94,7 +94,7 @@ End Absorption.
 
 Section Identity.
 
-Lemma lookup_mat_one {n} (i j : fin n) : mat_one@i@j = if i =? j then 1 else 0.
+Lemma lookup_mat_id {n} (i j : fin n) : mat_id@i@j = if i =? j then 1 else 0.
 Proof. apply lookup_mat_build. Qed.
 
 Lemma Σ_eqb_indicator (x : X) (n : nat) (j : fin n) :
@@ -106,21 +106,21 @@ rewrite Heq; apply Nat.eqb_refl. apply NoDup_vseq. apply elem_of_vseq.
 Qed.
 
 Theorem left_id_mat_mul {m n} (a : mat m n) :
-  mat_one × a ≡ a.
+  mat_id × a ≡ a.
 Proof.
 intros i j; erewrite lookup_mat_mul, equiv_Σ_fmap.
 apply Σ_eqb_indicator with (j:=i), fin_to_nat_lt.
-intros k _; rewrite lookup_mat_one, Nat.eqb_sym; destruct (k =? i) eqn:E.
+intros k _; rewrite lookup_mat_id, Nat.eqb_sym; destruct (k =? i) eqn:E.
 apply Nat.eqb_eq, fin_to_nat_inj in E; subst k.
 apply left_id; c. apply left_absorb; c.
 Qed.
 
 Theorem right_id_mat_mul {m n} (a : mat m n) :
-  a × mat_one ≡ a.
+  a × mat_id ≡ a.
 Proof.
 intros i j; erewrite lookup_mat_mul, equiv_Σ_fmap.
 apply Σ_eqb_indicator with (j:=j), fin_to_nat_lt.
-intros k _; rewrite lookup_mat_one; destruct (k =? j) eqn:E.
+intros k _; rewrite lookup_mat_id; destruct (k =? j) eqn:E.
 apply Nat.eqb_eq, fin_to_nat_inj in E; subst k.
 apply right_id; c. apply right_absorb; c.
 Qed.
@@ -195,7 +195,7 @@ End Distributivity.
 
 End Matrix_multiplication.
 
-Notation "a × b" := (mat_mul a b) (at level 40).
+Notation "a × b" := (mat_mul a b) (left associativity, at level 40).
 
 Section Matrix_semiring.
 
@@ -205,17 +205,17 @@ Notation mat := (mat X n n).
 
 Context `{SR : Semiring X}.
 
-Global Instance : One mat := mat_one.
+Global Instance : One mat := mat_id.
 Global Instance : Mul mat := mat_mul.
 
-Lemma mul_mat_unfold a b : a * b = a × b.
+Lemma mat_mul_fold a b : a × b = a * b.
 Proof. done. Qed.
 
-Lemma mat_one_fold : mat_one = 1.
+Lemma mat_id_fold : mat_id = 1.
 Proof. done. Qed.
 
 Lemma lookup_one i j : 1@i@j = if i =? j then 1 else 0.
-Proof. apply lookup_mat_one. Qed.
+Proof. apply lookup_mat_id. Qed.
 
 Global Instance : Semiring mat.
 Proof.
