asterate.v
@@ -16,40 +16,52 @@ Variable m n : nat.
 Variable star_m: sq m -> sq m.
 Variable star_n: sq n -> sq n.
 
+Notation "x '{m*}'":= (star_m x) (at level 31, format "x '{m*}'").
+Notation "x '{n*}'":= (star_n x) (at level 31, format "x '{n*}'").
+
 Definition mat_star_blocks
-  (a : sq m) (b : mat m n)
+  (a : sq m) (b : mat m n) 
   (c : mat n m) (d : sq n) : sq (m + n) :=
-  let d'     := star_n d     in
+  let d'     := d{n*}        in
   let bd'    := b × d'       in
   let d'c    := d' × c       in
   let f      := a + bd' × c  in
-  let f'     := star_m f     in
+  let f'     := f{m*}        in
   let f'bd'  := f' × bd'     in
   let d'cf'  := d'c × f'     in
   blocks f' f'bd' d'cf' (d' + d'cf' × bd').
 
-Hypothesis left_expand_star_m : ∀ a, star_m a ≡ 1 + a * star_m a.
-Hypothesis left_expand_star_n : ∀ a, star_n a ≡ 1 + a * star_n a.
+Hypothesis left_expand_star_m : ∀ a, a{m*} ≡ 1 + a * a{m*}.
+Hypothesis left_expand_star_n : ∀ a, a{n*} ≡ 1 + a * a{n*}.
+
+Local Ltac reduce :=
+  rewrite ?(left_id 0 add), ?(assoc add), ?assoc_mat_mul, ?mat_id_fold.
 
 Lemma left_expand_mat_star_blocks a b c d :
   mat_star_blocks a b c d ≡ 1 + blocks a b c d * mat_star_blocks a b c d.
 Proof.
 unfold mat_star_blocks.
-rewrite eq_one_blocks, mul_mat_unfold, equiv_mul_blocks, equiv_add_blocks.
-remember (a + (b × star_n d) × c) as f; apply proper_blocks.
-- rewrite assoc_mat_mul, <-right_distr_mat_mul, assoc_mat_mul, <-Heqf.
-  apply left_expand_star_m.
-- rewrite left_id, <-?assoc_mat_mul, assoc_mat_mul with (b:=c).
-  rewrite left_distr_mat_mul, assoc_mat_mul with (a:=b).
-  rewrite (assoc add), comm with (y:=b×_).
-  rewrite <-(assoc add), <-right_distr_mat_mul.
-  rewrite assoc_mat_mul with (a:=b), <-Heqf, assoc_mat_mul with (a:=f).
-  rewrite <-left_id_mat_mul with (a:=b×star_n d) at 2.
-  rewrite mat_one_fold, <-right_distr_mat_mul, <-mul_mat_unfold.
-  rewrite <-left_expand_star_m; reflexivity. all: c.
-- admit.
-- admit.
-Admitted.
+rewrite <-mat_mul_fold, eq_one_blocks, equiv_mul_blocks, equiv_add_blocks.
+remember (a + b × d{n*} × c) as f; apply proper_blocks; reduce.
+- rewrite <-(assoc add), <-right_distr_mat_mul.
+  rewrite <-Heqf; apply left_expand_star_m.
+- rewrite left_distr_mat_mul; reduce.
+  rewrite (comm add) with (y:=b×_), <-(assoc add).
+  rewrite <-left_id_mat_mul with (a:=b×_) at 1; rewrite mat_id_fold.
+  rewrite <-?right_distr_mat_mul, <-Heqf; reduce.
+  rewrite <-?right_distr_mat_mul, mat_mul_fold, <-left_expand_star_m; done.
+- rewrite <-left_id_mat_mul with (a:=c×_); reduce.
+  rewrite <-?right_distr_mat_mul, mat_mul_fold.
+  rewrite <-left_expand_star_n; done.
+- rewrite ?left_distr_mat_mul; reduce.
+  rewrite <-?(assoc add), <-?right_distr_mat_mul.
+  rewrite (comm add) with (x:=_×b), <-(assoc add), <-?right_distr_mat_mul.
+  rewrite <-left_id_mat_mul with (a:=c) at 3; reduce.
+  rewrite <-?right_distr_mat_mul, (comm add) with (y:=1).
+  rewrite ?mat_mul_fold, <-left_expand_star_n, <-?mat_mul_fold.
+  rewrite right_distr_mat_mul; reduce.
+  rewrite ?mat_mul_fold, <-left_expand_star_n; done.
+Qed.
 
 End Block_construction.
 
@@ -69,6 +81,12 @@ Fixpoint mat_star_ind {n} : sq n -> sq n :=
   | S m => mat_star_ind_step mat_star_ind
   end.
 
+Lemma mat_star_ind_S_unfold {n} (a : sq (S n)) :
+  mat_star_ind a = mat_star_ind_step mat_star_ind a.
+Proof.
+done.
+Qed.
+
 Lemma blocks_S_partition {n} (a : sq (S n)) :
   let p := mat_S_partition a in
   a = blocks p.1.1 p.1.2 p.2.1 p.2.2.
@@ -79,10 +97,13 @@ cbn; try done; intros; f_equal; rewrite vlookup_zip_with, ?vlookup_map; cbn.
 all: rewrite <-Vector.eta; reflexivity.
 Qed.
 
-Lemma mat_star_ind_S_unfold {n} (a : sq (S n)) :
-  mat_star_ind a = mat_star_ind_step mat_star_ind a.
+Ltac inv_fin_1 i := inv_fin i; [|intros i; inv_fin i].
+
+Lemma left_expand_mat_map_star (a : sq 1) :
+  mat_map star a ≡ 1 + a * mat_map star a.
 Proof.
-done.
+inv_vec a; intros a; inv_vec a; intros x i j; inv_fin_1 i; inv_fin_1 j; cbn.
+rewrite (right_id 0 add); apply left_expand_star.
 Qed.
 
 Lemma left_expand_mat_star_ind n (a : sq n) :
@@ -92,8 +113,8 @@ induction n. cbn; inv_vec a; done.
 rewrite blocks_S_partition with (a:=a) at 2.
 rewrite mat_star_ind_S_unfold; unfold mat_star_ind_step.
 rewrite left_expand_mat_star_blocks at 1.
-done. admit. apply IHn.
-Admitted.
+done. apply left_expand_mat_map_star. apply IHn.
+Qed.
 
 Lemma right_expand_mat_star_ind n (a : sq n) :
   mat_star_ind a ≡ 1 + mat_star_ind a * a.
